F= A'B'C'+A'BC'+A'BC+
AB'C + ABC

F = (A+B+C')(A'+B+C)(A+B+C')



A + AB = A
A(1 + B)
 A(1) = a

AA' =0

  CD 00  01  11  10
AB
00    0   0   0   0
01    0   1   1   0
11    1   1   1   1
10    0   1   1   1

  CD 00  01  11  10
AB    
00    1   1   1   1
01    1   1   1   1
11    1   1   1   1
10    1   1   1   1

F = A + AB + A'B + A'

  CD 00  01  11  10
AB    
00    0   0   0   0
01    0   0   0   0
11    1   1   1   1
10    1   1   1   1

F=A

  CD 00  01  11  10
AB    
00    0   0   1   1
01    0   0   1   1
11    1   1   1   1
10    1   1   1   1
F=A+C

  CD 00  01  11  10
AB    
00    1   1   0   0
01    1   1   0   0
11    0   0   1   1
10    0   0   1   1
F=A'C' + AC= A XNOR C

F = ABCD + ABC'D + AB'C + A'BCD
    (ABD)(1)
  CD 00  01  11  10
AB    
00    
01            1
11        1   1
10            1   1
F=BCD+ACD+ABD+AB'C 

  CD 00  01  11  10
AB    
00    1   0   0   1
01    1   0   0   1
11    1   0   0   1
10    1   0   0   1

F = C'D' + CD' = D(C+C') = D'

  CD 00  01  11  10
AB    
00    1   1   1   1
01    0   0   0   0
11    0   0   0   0
10    1   1   1   1
F=B'

  CD 00  01  11  10
AB    
00    0   0   0   0
01    1   1   1   1
11    1   1   1   1
10    1   1   1   1

F=A+B


  CD 00  01  11  10
AB    
00        1       1
01    1       1
11        1       1
10    1       1
